unique_ids2.thy
@@ -10,7 +10,6 @@ theory unique_ids2
     execution_invariants_unused
     impl_language
     topological_sort
-    unique_ids_procedure_check
 begin
 
 
@@ -33,13 +32,16 @@ definition
 \<forall>i r. ires i \<triangleq> r \<longrightarrow> uidv \<notin> uniqueIds r "
 
 definition
-"new_unique_not_in_other_invocations i los p uidv \<equiv>
-(\<forall>i' ls impl. i' \<noteq> i \<longrightarrow> los i' \<triangleq> ls \<longrightarrow> p i' \<triangleq> impl \<longrightarrow> (\<exists>uids. uidv \<notin> uids \<and> procedure_cannot_guess_ids uids ls impl))"
+"new_unique_not_in_other_invocations i S uidv \<equiv>
+(\<forall>i'. i' \<noteq> i \<longrightarrow> (\<exists>uids. uidv \<notin> uids \<and> invocation_cannot_guess_ids uids i' S))"
 
 
+lemmas use_new_unique_not_in_other_invocations = new_unique_not_in_other_invocations_def[THEN meta_eq_to_obj_eq, THEN iffD1, rule_format]
+
+(*
 lemma show_new_unique_not_in_other_invocations:
-  assumes a1: "new_unique_not_in_other_invocations i los p uidv"
-    and a2: "\<And>i' uids ls ls' impl. \<lbrakk>i' \<noteq> i; los i' \<triangleq> ls; los' i' \<triangleq> ls'; p i' \<triangleq> impl;  procedure_cannot_guess_ids uids ls impl\<rbrakk> \<Longrightarrow> procedure_cannot_guess_ids uids ls' impl"
+  assumes a1: "new_unique_not_in_other_invocations i S uidv"
+    and a2: "\<And>i' uids ls ls' impl. \<lbrakk>i' \<noteq> i; los i' \<triangleq> ls; los' i' \<triangleq> ls'; p i' \<triangleq> impl;  invocations_cannot_guess_ids uids ls impl\<rbrakk> \<Longrightarrow> procedure_cannot_guess_ids uids ls' impl"
     and a3: "dom los = dom los'"
   shows "new_unique_not_in_other_invocations i los' p uidv"
 proof (auto simp add: new_unique_not_in_other_invocations_def)
@@ -61,16 +63,17 @@ proof (auto simp add: new_unique_not_in_other_invocations_def)
   show "\<exists>uids.  uidv \<notin> uids \<and> procedure_cannot_guess_ids uids ls impl"
     using \<open>procedure_cannot_guess_ids uids ls impl\<close> b5 by auto
 qed
+*)
 
 definition uid_is_private where
-"uid_is_private i s_calls s_invocationOp s_invocationRes s_knownIds s_generatedIds s_localState s_currentProc uidv  \<equiv> 
-      new_unique_not_in_invocationOp s_invocationOp uidv
-    \<and> new_unique_not_in_calls s_calls uidv
-    \<and> new_unique_not_in_calls_result s_calls uidv
-    \<and> new_unique_not_in_invocationRes s_invocationRes uidv
-    \<and> uidv \<notin> s_knownIds
-    \<and> s_generatedIds uidv \<triangleq> i
-    \<and> new_unique_not_in_other_invocations i s_localState s_currentProc uidv"
+"uid_is_private i S uidv  \<equiv> 
+      new_unique_not_in_invocationOp (invocationOp S) uidv
+    \<and> new_unique_not_in_calls (calls S) uidv
+    \<and> new_unique_not_in_calls_result (calls S) uidv
+    \<and> new_unique_not_in_invocationRes (invocationRes S) uidv
+    \<and> uidv \<notin> (knownIds S)
+    \<and> generatedIds S uidv \<triangleq> i
+    \<and> new_unique_not_in_other_invocations i S uidv"
 
 
 definition uid_is_private' where
@@ -82,23 +85,22 @@ definition uid_is_private' where
     \<and> uidv \<notin> s_knownIds
     "
 lemma uid_is_private'_implies:
-"uid_is_private i s_calls s_invocationOp s_invocationRes s_knownIds s_generatedIds s_localState s_currentProc uidv
- \<Longrightarrow> uid_is_private' i s_calls s_invocationOp s_invocationRes s_knownIds uidv"
+"uid_is_private i S uidv
+ \<Longrightarrow> uid_is_private' i (calls S) (invocationOp S) (invocationRes S) (knownIds S) uidv"
   by (auto simp add: uid_is_private_def uid_is_private'_def)
 
 
 lemma growth_still_hidden_step_other:
   assumes S_wf: "state_wellFormed S"
     and prog_wf: "program_wellFormed (prog S)"
-    and p1: "uid_is_private i (calls S) (invocationOp S) (invocationRes S) (knownIds S) (generatedIds S) (localState S) (currentProc S) uidv"
+    and p1: "uid_is_private i S uidv"
     and step: "S ~~ (i', a) \<leadsto> S'"
     and other: "i' \<noteq> i"
-  shows "uid_is_private i (calls S') (invocationOp S') (invocationRes S') (knownIds S') (generatedIds S') (localState S') (currentProc S') uidv"
+  shows "uid_is_private i S' uidv"
 proof -
 
 
-  have priv_S: "uid_is_private i (calls S) (invocationOp S) (invocationRes S) (knownIds S) (generatedIds S) (localState S)
-         (currentProc S) uidv"
+  have priv_S: "uid_is_private i S uidv"
     by (simp add: p1)
 
 
@@ -114,20 +116,53 @@ proof -
     by (meson priv_S uid_is_private_def)
   have i5: "uidv \<notin> knownIds S"
     by (meson priv_S uid_is_private_def)
-  have i6: "new_unique_not_in_other_invocations i (localState S) (currentProc S) uidv"
+  have i6: "new_unique_not_in_other_invocations i S uidv"
     by (meson priv_S uid_is_private_def)
 
   have still_generated: "generatedIds S uidv \<triangleq> i"
     by (meson priv_S uid_is_private_def)
 
 
-  note invs = i1 i2 i3 i4 i5 i6 still_generated
+  have inv6': "new_unique_not_in_other_invocations i S' uidv"
+    if "uidv \<notin> action_inputs a"
+    unfolding new_unique_not_in_other_invocations_def 
+  proof (intro allI impI)
+    fix i''
+    assume a0: "i'' \<noteq> i"
+
+    obtain uids where "uidv \<notin> uids" and "invocation_cannot_guess_ids uids i'' S"
+      by (metis a0 i6 new_unique_not_in_other_invocations_def)
 
 
+    show "\<exists>uids. uidv \<notin> uids \<and> invocation_cannot_guess_ids uids i'' S'"
+    proof (cases "i'' = i'")
+      case True
 
-  have i6': "\<And>ls impl. localState S i' \<triangleq> ls \<Longrightarrow> currentProc S i' \<triangleq> impl \<Longrightarrow> (\<exists>uids.  uidv \<notin> uids \<and> procedure_cannot_guess_ids uids ls impl)"
-    using \<open>i' \<noteq> i\<close> i6
-    by (meson new_unique_not_in_other_invocations_def) 
+      from `invocation_cannot_guess_ids uids i'' S`
+      have "invocation_cannot_guess_ids (uids \<union> action_inputs a) i'' S'"
+      proof (rule show_invocation_cannot_guess_ids_step)
+        show "S ~~ (i'', a) \<leadsto> S'"
+          by (simp add: True local.step)
+      qed
+
+      then show ?thesis
+        using UnE \<open>uidv \<notin> uids\<close> that by auto
+    next
+      case False
+
+      from `invocation_cannot_guess_ids uids i'' S` step
+      have "invocation_cannot_guess_ids uids i'' S'"
+        by (rule show_invocation_cannot_guess_ids_step_other, use False in simp)
+
+      then show ?thesis
+        using \<open>uidv \<notin> uids\<close> by blast
+    qed
+  qed
+
+
+  note invs = i1 i2 i3 i4 i5 i6 inv6' still_generated
+
+
 
 
 
@@ -135,6 +170,7 @@ proof -
     using S_wf local.step noFail state_wellFormed_combine1 by blast
 
 
+  
 
 
   from `S ~~ (i', a) \<leadsto> S'`
@@ -142,46 +178,41 @@ proof -
   proof (induct rule: step.cases)
     case (local S i2 ls f ls')
 
-    obtain uids where  uids1: " uidv \<notin> uids" and uids2: "procedure_cannot_guess_ids uids ls f"
-      using \<open>i' \<noteq> i\<close> i6 local i6' by auto 
 
     from local
     show ?case
-      using invs  apply (auto simp add: uid_is_private_def elim!: show_new_unique_not_in_other_invocations split: if_splits)
-      by (meson pcgi_local_case uids1 uids2)
-
-
+      using invs by (auto simp add: uid_is_private_def  split: if_splits)
 
   next
     case (newId S i' ls f ls' uid uidv ls'')
     show ?case 
-      using invs  apply (auto simp add: uid_is_private_def newId)
-      using `uid = to_nat uidv` `generatedIds S uid = None` apply auto[1]
-      using `uid = to_nat uidv` `generatedIds S uid = None`  apply (auto simp add: new_unique_not_in_other_invocations_def)
-      by (metis (no_types, lifting) Un_insert_right insert_iff newId.hyps(4) newId.hyps(5) newId.hyps(6) newId.hyps(8) newId.hyps(9) option.inject pcgi_newId_case sup_bot.comm_neutral)
-
+      using invs  `uid = to_nat uidv` `generatedIds S uid = None` newId by (auto simp add: uid_is_private_def)
 
   next
     case (beginAtomic S i ls f ls' t vis snapshot)
-    then show ?case using invs by (auto simp add: uid_is_private_def pcgi_beginAtomic_case elim!: show_new_unique_not_in_other_invocations split: if_splits)
+    then show ?case using invs by (auto simp add: uid_is_private_def  split: if_splits)
   next
     case (endAtomic S i ls f ls' t)
     then show ?case using invs 
-      by (auto simp add: uid_is_private_def pcgi_endAtomic_case elim!: show_new_unique_not_in_other_invocations split: if_splits)
-
-
-
+      by (auto simp add: uid_is_private_def   split: if_splits)
 
   next
     case (dbop S i' ls f Op ls' t c res vis)
 
-    obtain uids where  uids1: " uidv \<notin> uids" and uids2: "procedure_cannot_guess_ids uids ls f"
-      using dbop.hyps(1) dbop.hyps(2) dbop.hyps(4) dbop.hyps(5) i6' by blast 
+    have "i' \<noteq> i"
+      using dbop.hyps(2) other by blast
+
+
+    obtain uids where  uids1: " uidv \<notin> uids" and uids2: "invocation_cannot_guess_ids uids i' S"
+      by (metis \<open>i' \<noteq> i\<close> dbop.hyps(1) i6 new_unique_not_in_other_invocations_def)
+
+
+    from uids2 step
+    have "uniqueIds Op \<subseteq> uids" 
+      by (fuzzy_rule use_invocation_cannot_guess_ids_dbop, use dbop in auto)
 
 
 
-    from pcgi_dbop_case1[OF uids2 `f ls = DbOperation Op ls'`]
-    have "uniqueIds Op \<subseteq> uids" .
 
     with uids1 have uids2: " uidv \<notin> uniqueIds Op"
       by auto
@@ -208,51 +239,34 @@ proof -
 
 
     show ?case 
-    proof (auto simp add: uid_is_private_def dbop invs uids2 uids3 )
-      show "new_unique_not_in_invocationOp (invocationOp S) uidv"
-        using dbop.hyps(1) i1 by blast
-
-
-      show "new_unique_not_in_calls (calls S(c \<mapsto> Call Op res)) uidv"
-        using uids2 i2 by (auto simp add: new_unique_not_in_calls_def dbop )
-
-      show " new_unique_not_in_calls_result (calls S(c \<mapsto> Call Op res)) uidv"
-        using uids2 i3 by (auto simp add: new_unique_not_in_calls_result_def dbop uids3)
-
-
-      show "new_unique_not_in_invocationRes (invocationRes S) uidv"
-        using dbop.hyps(1) i4 by blast
-
-      show " uidv \<in> knownIds S \<Longrightarrow> False"
-        using dbop.hyps(1) i5 by blast
-
-      show "new_unique_not_in_other_invocations i (localState S(i' \<mapsto> ls' res)) (currentProc S) uidv"
-        by (smt UnE \<open>\<And>thesis. (\<And>uids. \<lbrakk>uidv \<notin> uids; procedure_cannot_guess_ids uids ls f\<rbrakk> \<Longrightarrow> thesis) \<Longrightarrow> thesis\<close> dbop.hyps(1) dbop.hyps(5) dbop.hyps(6) fun_upd_other fun_upd_same i6 new_unique_not_in_other_invocations_def option.sel pcgi_dbop_case2 uids3)
-
-
-      show "generatedIds S uidv \<triangleq> i"
-        using dbop.hyps(1) still_generated by blast
-
+      unfolding uid_is_private_def
+    proof (intro conjI)
+      show "new_unique_not_in_invocationOp (invocationOp S') uidv"
+        using dbop.hyps(1) i1 by (auto simp add: dbop)
+      show "new_unique_not_in_calls (calls S') uidv"
+        using dbop.hyps(1) i2 by (auto simp add: dbop new_unique_not_in_calls_def uids2)
+      show "new_unique_not_in_calls_result (calls S') uidv"
+        using dbop.hyps(1) i3 by (auto simp add: dbop new_unique_not_in_calls_result_def uids3)
+      show "new_unique_not_in_invocationRes (invocationRes S') uidv"
+       using dbop.hyps(1) i4 by (auto simp add: dbop)
+      show "uidv \<notin> knownIds S'"
+        using dbop.hyps(1) i5  by (auto simp add: dbop)
+      show "generatedIds S' uidv \<triangleq> i"
+        using dbop.hyps(1) still_generated by (auto simp add: dbop)
+      show "new_unique_not_in_other_invocations i S' uidv "
+        using dbop.hyps(2) inv6' uids3 by auto
     qed
-
-
-
-
 
   next
     case (invocation S i proc initialState impl)
-    then show ?case using invs apply (auto simp add: uid_is_private_def)
-       apply (auto simp add: new_unique_not_in_invocationOp_def)
-      apply (auto simp add: new_unique_not_in_other_invocations_def)
-      by (metis prog_wf program_wellFormed_def show_procedures_cannot_guess_ids subsetD subset_Un_eq subset_refl)
+    then show ?case using invs by (auto simp add: uid_is_private_def new_unique_not_in_invocationOp_def)
 
   next
     case (return S i ls f res)
     then show ?case using invs apply (auto simp add: uid_is_private_def)
-        apply (auto simp add: new_unique_not_in_invocationRes_def)
-      using i6' pcgi_return_case apply fastforce
-      using i6' pcgi_return_case apply fastforce
-      by (simp add: new_unique_not_in_other_invocations_def)
+       apply (auto simp add: new_unique_not_in_invocationRes_def)
+      apply (metis action_outputs.simps(7) i6 invocation_cannot_guess_ids_step local.step new_unique_not_in_other_invocations_def other )
+      by (metis action_outputs.simps(7) i6 invocation_cannot_guess_ids_step local.step new_unique_not_in_other_invocations_def other)
 
   next
     case (fail S i ls)
@@ -271,11 +285,11 @@ qed
 lemma growth_still_hidden_steps_other:
   assumes S_wf: "state_wellFormed S"
     and prog_wf: "program_wellFormed (prog S)"
-    and p1: "uid_is_private i (calls S) (invocationOp S) (invocationRes S) (knownIds S) (generatedIds S) (localState S) (currentProc S) uidv"
+    and p1: "uid_is_private i S uidv"
     and steps: "S ~~ tr \<leadsto>* S'"
     and other: "\<forall>(i',a)\<in>set tr. i' \<noteq> i"
     and no_fail: "\<forall>i. (i, ACrash) \<notin> set tr"
-  shows "uid_is_private i (calls S') (invocationOp S') (invocationRes S') (knownIds S') (generatedIds S') (localState S') (currentProc S') uidv"
+  shows "uid_is_private i S' uidv"
 using steps   p1 other no_fail proof (induct rule: steps_induct)
   case initial
   then show ?case by simp
@@ -293,8 +307,7 @@ next
       using local.step by auto
     show "program_wellFormed (prog S')"
       using prog_wf step.steps steps_do_not_change_prog by fastforce
-    show "uid_is_private i (calls S') (invocationOp S') (invocationRes S') (knownIds S') (generatedIds S') (localState S')
-     (currentProc S') uidv"
+    show "uid_is_private i S' uidv"
       using step by auto
   qed
 qed
@@ -304,8 +317,8 @@ qed
 lemma growth_still_hidden:
   assumes g: "state_monotonicGrowth i S S'"
     and prog_wf: "program_wellFormed (prog S)"
-    and p1: "uid_is_private i (calls S) (invocationOp S) (invocationRes S) (knownIds S) (generatedIds S) (localState S) (currentProc S) uidv"
-  shows "uid_is_private i (calls S') (invocationOp S') (invocationRes S') (knownIds S') (generatedIds S') (localState S') (currentProc S') uidv"
+    and p1: "uid_is_private i S uidv"
+  shows "uid_is_private i S' uidv"
 proof -
   from g obtain tr
     where wf: "state_wellFormed S"
@@ -320,6 +333,163 @@ proof -
     using growth_still_hidden_steps_other by blast
 qed
 
+lemma step_to_steps:
+  assumes "S ~~ a \<leadsto> S'"
+  shows " S ~~ [a] \<leadsto>* S'"
+  by (simp add: assms steps_single)
 
+
+lemma step_to_steps_ex:
+  assumes "S ~~ a \<leadsto> S'"
+  shows "\<exists>tr. S ~~ tr \<leadsto>* S'"
+  by (rule exI[where x="[a]"], simp add: assms steps_single)
+
+lemma step_s_to_step:
+  assumes steps_s: "S ~~ (i, a, ok) \<leadsto>\<^sub>S S'"
+    and no_AInvoc: "\<And>p. a \<noteq> AInvoc p"
+    and no_beginAtomic: "\<And>t txns. a \<noteq> ABeginAtomic t txns"
+  shows steps: " S ~~ (i, a) \<leadsto> S'"
+  using steps_s proof cases
+  case (local ls f ls')
+  thus "S ~~ (i, a) \<leadsto> S'"
+    by (auto simp add: step.simps)
+next
+  case (newId ls f ls' uid uidv ls'')
+  thus "S ~~ (i, a) \<leadsto> S'"
+    by (auto simp add: step.simps)
+next
+  case (beginAtomic ls f ls' t S'a vis vis')
+  thus ?thesis using no_beginAtomic by auto
+next
+  case (endAtomic ls f ls' t)
+  thus "S ~~ (i, a) \<leadsto> S'"
+    by (auto simp add: step.simps)
+next
+  case (dbop ls f Op ls' t c res vis)
+  thus "S ~~ (i, a) \<leadsto> S'"
+    by (auto simp add: step.simps)
+next
+  case (invocation proc initState impl S')
+  with no_AInvoc have False by auto
+  thus ?thesis
+    ..
+next
+  case (return ls f res)
+  thus "S ~~ (i, a) \<leadsto> S'"
+    by (auto simp add: step.simps)
+qed
+
+lemma step_s_beginAtomic_to_steps:
+  assumes step_s: "S ~~ (i, ABeginAtomic t txns, ok) \<leadsto>\<^sub>S S'"
+  shows "\<exists>Sx tr. (S ~~ tr \<leadsto>* Sx) \<and> (\<forall>(i',a)\<in>set tr.  i' \<noteq> i) \<and> (\<forall>i. (i, ACrash) \<notin> set tr)  \<and>  Sx ~~ (i, ABeginAtomic t txns) \<leadsto> S'"
+  using assms proof cases
+  case (beginAtomic ls f ls' S'a vis)
+
+  from `state_monotonicGrowth i S S'a`
+  obtain tr where x1: "S ~~ tr \<leadsto>* S'a"
+    and x2: "\<forall>(i',a)\<in>set tr.  i' \<noteq> i"
+    and x3: "\<forall>i. (i, ACrash) \<notin> set tr"
+    by (auto simp add: state_monotonicGrowth_def)
+
+  have "S'a ~~ (i, ABeginAtomic t txns) \<leadsto> S'"
+    using beginAtomic by (auto simp add: step.simps)
+
+
+
+  with x1 x2 x3
+  show ?thesis 
+    using steps_step by blast
+qed
+
+lemma  show_invocation_cannot_guess_ids_steps_other: 
+  assumes icgi: "invocation_cannot_guess_ids uids i S" 
+    and steps: "S ~~ tr \<leadsto>* S'"
+    and other: "\<forall>(i',a)\<in>set tr. i' \<noteq> i"
+  shows "invocation_cannot_guess_ids uids i S'" 
+  using steps icgi other 
+proof (induct rule: steps_induct)
+case initial
+  then show ?case
+    by simp
+next
+  case (step S' tr a S'')
+  then show ?case
+    using show_invocation_cannot_guess_ids_step_other
+    by (smt Un_iff case_prodE insert_iff list.set(1) list.set(2) prod.sel(1) set_append )
+qed
+
+
+lemma  show_invocation_cannot_guess_ids_step_s_other: 
+  assumes "invocation_cannot_guess_ids uids i S" 
+    and step: "S ~~ (i', a) \<leadsto>\<^sub>S S'"
+    and "i' \<noteq> i"
+    and no_beginAtomic: "\<And>t txns. fst a \<noteq> ABeginAtomic t txns"
+    and no_AInvoc: "\<And>p. fst a \<noteq> AInvoc p"
+  shows "invocation_cannot_guess_ids uids i S'" 
+proof -
+  have "S ~~ (i', fst a) \<leadsto> S'"
+  proof (rule step_s_to_step)
+    show "S ~~ (i', fst a, snd a) \<leadsto>\<^sub>S S'"
+      using step by simp
+  qed (simp add: no_AInvoc no_beginAtomic)+
+
+  with `invocation_cannot_guess_ids uids i S`
+  show "invocation_cannot_guess_ids uids i S'"
+    using `i' \<noteq> i` show_invocation_cannot_guess_ids_step_other by blast
+qed
+
+
+lemma invocation_cannot_guess_ids_steps:
+  assumes "invocation_cannot_guess_ids uids i S"
+    and "S ~~ tr \<leadsto>* S'"
+  shows "invocation_cannot_guess_ids (uids \<union> trace_inputs tr i) i S'"
+proof (rule show_invocation_cannot_guess_ids)
+  fix x tra a S'a
+  assume a0: "S' ~~ tra @ [(i, a)] \<leadsto>* S'a"
+    and a1: "x \<in> action_outputs a"
+    and a2: "x \<notin> uids \<union> trace_inputs tr i"
+
+  have "S ~~ ((tr@tra) @ [(i,a)]) \<leadsto>* S'a"
+    using a0 assms(2) steps_append2 by force
+
+
+  from use_invocation_cannot_guess_ids[OF  `invocation_cannot_guess_ids uids i S` `S ~~ ((tr@tra) @ [(i,a)]) \<leadsto>* S'a`]
+  have "trace_outputs ((tr @ tra) @ [(i, a)]) i \<subseteq> trace_inputs (tr @ tra) i \<union> uids" .
+  hence "action_outputs a \<subseteq> trace_inputs (tr @ tra) i \<union> uids"
+    by (auto simp add: trace_outputs_def)
+
+  with `x \<in> action_outputs a` `x \<notin> uids \<union> trace_inputs tr i`
+  show "x \<in> trace_inputs tra i"
+    by (auto simp add: trace_inputs_append)
+qed
+
+lemma new_unique_not_in_other_invocations_maintained:
+  assumes "new_unique_not_in_other_invocations i S x"
+    and "S ~~ (i, action, Inv) \<leadsto>\<^sub>S S'"
+    and no_AInvoc: "\<And>p. action \<noteq> AInvoc p"
+    and no_beginAtomic: "\<And>t txns. action \<noteq> ABeginAtomic t txns"
+  shows "new_unique_not_in_other_invocations i S' x"
+  unfolding new_unique_not_in_other_invocations_def
+proof (intro allI impI)
+  fix i'
+  assume a0: "i' \<noteq> i"
+
+  obtain uids where "x \<notin> uids" and "invocation_cannot_guess_ids uids i' S"
+    by (meson a0 assms(1) new_unique_not_in_other_invocations_def)
+
+
+  from `S ~~ (i, action, Inv) \<leadsto>\<^sub>S S'`
+  have "S ~~ (i, action) \<leadsto> S'"
+    by (simp add: no_AInvoc no_beginAtomic step_s_to_step)
+
+
+  have "invocation_cannot_guess_ids uids i' S'"
+
+    using \<open>S ~~ (i, action) \<leadsto> S'\<close> \<open>invocation_cannot_guess_ids uids i' S\<close> a0 show_invocation_cannot_guess_ids_step_other by blast
+
+
+  thus "\<exists>uids. x \<notin> uids \<and> invocation_cannot_guess_ids uids i' S'"
+    using \<open>x \<notin> uids\<close> by blast
+qed
 
 end
