unique_ids_procedure_check.thy
@@ -40,4 +40,154 @@ definition procedures_cannot_guess_ids :: "('proc::valueType \<Rightarrow> ('ls 
 
 lemmas show_procedures_cannot_guess_ids = procedures_cannot_guess_ids_def[THEN iffD1, rule_format]
 
+
+lemma pscgi_to_iscgi:
+  assumes "procedures_cannot_guess_ids (procedure progr)"
+  shows "invocations_cannot_guess_ids progr"
+  unfolding invocations_cannot_guess_ids_def invocation_cannot_guess_ids_def
+proof (intro allI impI)
+
+  fix i1 tr1 a S'
+  assume steps: "initialState progr ~~ tr1 @ [a] \<leadsto>* S'"
+
+  define tr1a where "tr1a = tr1@[a]"
+
+  from steps
+  have "initialState progr ~~ tr1a \<leadsto>* S'"
+    using tr1a_def by blast
+
+  value "butlast [1,2,3::nat]"
+
+  from this 
+  have "trace_outputs tr1a i1 \<subseteq> trace_inputs (butlast tr1a) i1
+    \<and> (\<forall>ls impl. localState S' i1 \<triangleq> ls 
+        \<longrightarrow>  currentProc S' i1 \<triangleq> impl 
+        \<longrightarrow> procedure_cannot_guess_ids (trace_inputs tr1a i1) ls impl)"
+  proof (induct rule: steps_induct)
+    case initial
+    then show ?case
+      by (auto simp add: initialState_def trace_outputs_def)
+
+  next
+    case (step S' tr a S'')
+
+    have IH1: "trace_outputs tr i1 \<subseteq> trace_inputs (butlast tr) i1"
+      using step by auto
+
+    hence IH1': "trace_outputs tr i1 \<subseteq> trace_inputs tr i1"
+      by (induct tr rule: rev_induct, auto simp add:  trace_inputs_append)
+
+    have IH2: "procedure_cannot_guess_ids (trace_inputs tr i1) ls impl "
+      if "localState S' i1 \<triangleq> ls"
+        and "currentProc S' i1 \<triangleq> impl"
+      for ls impl
+      using step that by blast
+
+
+
+    show ?case
+    proof (cases "get_invoc a = i1")
+      case False
+      have [simp]: "trace_inputs (tr @ [a]) i1 = trace_inputs tr i1"
+        by (simp add: False trace_inputs_def)
+      have [simp]: "trace_outputs (tr @ [a]) i1 = trace_outputs tr i1"
+        by (simp add: False trace_outputs_def)
+
+      show ?thesis
+        using IH1' IH2 apply (auto simp add: step)
+        by (metis False IH2 prod.collapse step.step unchangedInTransaction(1) unchangedInTransaction(2))
+    next
+      case True
+
+
+
+      from `S' ~~ a \<leadsto> S''`
+      have "action_outputs (get_action a) \<subseteq> trace_inputs tr i1" 
+      proof cases
+        case (dbop i ls f Op ls' t c res vis)
+        have pcgi: "procedure_cannot_guess_ids (trace_inputs tr i1) ls f"
+          using True local.dbop(1) local.dbop(3) local.dbop(4) step.IH by auto
+
+        from pcgi_dbop_case1[OF pcgi `f ls = DbOperation Op ls'`]
+        have " uniqueIds Op \<subseteq> trace_inputs tr i1" .
+        then show ?thesis 
+          by (auto simp add: `a = (i, ADbOp c Op res)` trace_outputs_empty)
+      next
+        case (return i ls f res)
+        have pcgi: "procedure_cannot_guess_ids (trace_inputs tr i1) ls f"
+          using IH2 True local.return(1) local.return(3) local.return(4) by auto
+
+        from pcgi_return_case[OF pcgi]
+        show ?thesis
+          by (auto simp add: return)
+      qed auto
+
+      have [simp]: "(trace_inputs (tr @ [(i, action)]) i1)
+          = trace_inputs tr i1 \<union> (if i = i1 then action_inputs action else {})" for i action
+        by (auto simp add: trace_inputs_append trace_inputs_cons trace_inputs_empty)
+
+      from `S' ~~ a \<leadsto> S''`
+      have "procedure_cannot_guess_ids (trace_inputs (tr @ [a]) i1) ls impl"
+        if l1: "localState S'' i1 \<triangleq> ls"
+        and l2: "currentProc S'' i1 \<triangleq> impl"
+      for ls impl
+      proof cases
+        case (local i ls f ok ls')
+        then show ?thesis
+          using IH2 l1 l2 apply (auto simp add:  split: if_splits)
+          by (meson pcgi_local_case)
+      next
+        case (newId i ls f ls' uid uidv ls'')
+        then show ?thesis 
+          using IH2 l1 l2 apply (auto simp add:  split: if_splits)
+          using pcgi_newId_case by fastforce
+      next
+        case (beginAtomic i ls f ls' t vis snapshot)
+        then show ?thesis 
+          using IH2 l1 l2 apply (auto simp add:  split: if_splits)
+          by (meson pcgi_beginAtomic_case)
+      next
+        case (endAtomic i ls f ls' t)
+        then show ?thesis 
+          using IH2 l1 l2 apply (auto simp add:  split: if_splits)
+          by (meson pcgi_endAtomic_case)
+      next
+        case (dbop i ls f Op ls' t c res vis)
+        then show ?thesis 
+          using IH2 l1 l2 apply (auto simp add:  split: if_splits)
+          by (meson pcgi_dbop_case2)
+      next
+        case (invocation i proc initialState impl)
+        from  `procedures_cannot_guess_ids (procedure progr)`
+        have "procedure_cannot_guess_ids (uniqueIds proc) initialState impl"
+          apply (auto simp add: procedures_cannot_guess_ids_def)
+          by (metis (no_types, lifting) distributed_state.select_convs(1) initialState_def local.invocation(4) step.steps steps_do_not_change_prog sup.idem)
+
+        from invocation
+        show ?thesis 
+          using IH2 l1 l2 apply (auto simp add:  split: if_splits)
+          by (metis (no_types, lifting) assms distributed_state.select_convs(1) initialState_def show_procedures_cannot_guess_ids step.steps steps_do_not_change_prog)
+      next
+        case (return i ls f res)
+        then show ?thesis 
+          using IH2 l1 l2 by (auto simp add:  split: if_splits)
+      next
+        case (fail i ls)
+        then show ?thesis 
+          using IH2 l1 l2 by (auto simp add:  split: if_splits)
+      next
+        case (invCheck res i)
+        then show ?thesis 
+          using IH2 l1 l2 by (auto simp add:  split: if_splits)
+      qed
+
+      thus ?thesis
+        using  IH1' \<open>action_outputs (get_action a) \<subseteq> trace_inputs tr i1\<close> by (auto simp add: trace_outputs_append True subsetD trace_outputs_cons trace_outputs_empty)
+    qed
+  qed
+  thus "trace_outputs (tr1 @ [a]) i1 \<subseteq> trace_inputs tr1 i1 \<union> {}"
+    by (simp add: tr1a_def)
+qed
+
+
 end
